feat(library/init): add d_array type
@kha I added the `d_array` type that we discussed today.
However, the VM implemantion is still using persistent arrays.
If we remove the persistent array support, then code using
hash_map will only be efficient if the hash_map is used linearly.
This is not the case in the reader module because we are planning
to support backtracking.

On the other hand, it is awkward we currently don't have a vanilla
array implementation in the VM. I suspect this will be a problem in
the future.

So, I see the following possibilities:

1- We implement a map data-structure using red-black trees in Lean.
We use this new data-structure to implement all maps in the new reader and
macro expander.

2- We implement a very simple map as a list of pairs.
Then, we replace it in the VM with an efficient implementation.
The VM implementation may use our internal red-black trees.
We may also use a persistent hash table implemented in C++,
but it would be awkward to ask the user to provide a hash function in the reference
implementation (i.e., the one using list of pairs), but not use it
anywhere :)
In contrast, if we use the red-black tree implementation we
would have to ask the user to provide a total order.
It is overkill for the list of pair reference implementation because
we just need an equality test, but, at least, the comparison function
will be used in the implementation.

3- Add types `d_parray` (dependent persistent array) and
`parray` (persistent array). In Lean, they would just wrap the
`d_array` and `array` types. In the VM, `d_array` and `array` would
be implemented using vanilla arrays and `d_parray` and `parray` would
be implemented using persistent arrays. Then, we could have
`d_hash_map`, `hash_map`, `d_phash_map` and `phash_map`. Argh, so many
versions :(
We would use `phash_map` to implement our reader and macro expander.

4- Add a `(persistent : bool := ff)` parameter to `d_array` and
`array` types. The disadvantage of this approach is that it has
a performance impact. The VM implementation would have to check
the `persisent` flag at runtime. The value of this flag is known
at compilation time, but we currently don't have a mechanism
for specializing native builtin C++ implementations for VM functions.

src/library/vm/vm_array.cpp
@@ -63,7 +63,7 @@ vm_obj to_obj(parray<vm_obj> const & a) {
     return mk_vm_external(new (get_vm_allocator().allocate(sizeof(vm_array))) vm_array(a));
 }
 
-vm_obj array_read(vm_obj const &, vm_obj const &, vm_obj const & a, vm_obj const & i) {
+vm_obj d_array_read(vm_obj const &, vm_obj const &, vm_obj const & a, vm_obj const & i) {
     /* TODO(Leo): handle case where n is too big */
     unsigned idx = force_to_unsigned(i);
     lean_vm_check(idx < to_array(a).size());
@@ -71,7 +71,7 @@ vm_obj array_read(vm_obj const &, vm_obj const &, vm_obj const & a, vm_obj const
     return _a[idx];
 }
 
-vm_obj array_write(vm_obj const &, vm_obj const &, vm_obj const & a, vm_obj const & i, vm_obj const & v) {
+vm_obj d_array_write(vm_obj const &, vm_obj const &, vm_obj const & a, vm_obj const & i, vm_obj const & v) {
     /* TODO(Leo): handle case where n is too big */
     unsigned idx = force_to_unsigned(i);
     parray<vm_obj> const & p = to_array(a);
@@ -110,14 +110,14 @@ vm_obj array_pop_back(vm_obj const &, vm_obj const &, vm_obj const & a) {
     }
 }
 
-vm_obj mk_array(vm_obj const &, vm_obj const & n, vm_obj const & v) {
+vm_obj mk_array(vm_obj const & /* alpha */, vm_obj const & n, vm_obj const & v) {
     /* TODO(Leo): handle case where n is too big */
     unsigned _n = force_to_unsigned(n);
     parray<vm_obj> a(_n, v);
     return to_obj(a);
 }
 
-vm_obj array_mk(vm_obj const &, vm_obj const & n, vm_obj const & fn) {
+vm_obj d_array_mk(vm_obj const & n, vm_obj const & /* alpha */, vm_obj const & fn) {
     /* TODO(Leo): handle case where n is too big */
     unsigned _n = force_to_unsigned(n);
     parray<vm_obj> a;
@@ -127,7 +127,7 @@ vm_obj array_mk(vm_obj const &, vm_obj const & n, vm_obj const & fn) {
     return to_obj(a);
 }
 
-vm_obj array_foreach(vm_obj const &, vm_obj const & n, vm_obj const & a, vm_obj const & fn) {
+vm_obj d_array_foreach(vm_obj const & n, vm_obj const & /* alpha */, vm_obj const & a, vm_obj const & fn) {
     /* TODO(Leo): handle case where n is too big */
     unsigned _n = force_to_unsigned(n);
     parray<vm_obj> const & p = to_array(a);
@@ -145,8 +145,8 @@ vm_obj array_foreach(vm_obj const &, vm_obj const & n, vm_obj const & a, vm_obj 
     }
 }
 
-vm_obj array_iterate(vm_obj const &, vm_obj const &, vm_obj const & n,
-                     vm_obj const & a, vm_obj const & b, vm_obj const & fn) {
+vm_obj d_array_iterate(vm_obj const & n, vm_obj const & /* alpha */, vm_obj const & /* beta */,
+                       vm_obj const & a, vm_obj const & b, vm_obj const & fn) {
     /* TODO(Leo): handle case where n is too big */
     unsigned _n = force_to_unsigned(n);
     parray<vm_obj> const & p = to_array(a);
@@ -158,7 +158,7 @@ vm_obj array_iterate(vm_obj const &, vm_obj const &, vm_obj const & n,
 
 static unsigned g_array_read_idx = -1;
 
-unsigned array_cases_on(vm_obj const & o, buffer<vm_obj> & data) {
+unsigned d_array_cases_on(vm_obj const & o, buffer<vm_obj> & data) {
     vm_obj d[3] = {o, mk_vm_unit(), mk_vm_unit()};
     vm_obj fn = mk_vm_closure(g_array_read_idx, 3, d);
     data.push_back(fn);
@@ -166,22 +166,22 @@ unsigned array_cases_on(vm_obj const & o, buffer<vm_obj> & data) {
 }
 
 void initialize_vm_array() {
-    DECLARE_VM_BUILTIN(name({"array", "mk"}),               array_mk);
+    DECLARE_VM_BUILTIN(name({"d_array", "mk"}),             d_array_mk);
     DECLARE_VM_BUILTIN(name({"mk_array"}),                  mk_array);
-    DECLARE_VM_BUILTIN(name({"array", "data"}),             array_read);
-    DECLARE_VM_BUILTIN(name({"array", "read"}),             array_read);
-    DECLARE_VM_BUILTIN(name({"array", "write"}),            array_write);
+    DECLARE_VM_BUILTIN(name({"d_array", "data"}),           d_array_read);
+    DECLARE_VM_BUILTIN(name({"d_array", "read"}),           d_array_read);
+    DECLARE_VM_BUILTIN(name({"d_array", "write"}),          d_array_write);
     DECLARE_VM_BUILTIN(name({"array", "push_back"}),        array_push_back);
     DECLARE_VM_BUILTIN(name({"array", "pop_back"}),         array_pop_back);
-    DECLARE_VM_BUILTIN(name({"array", "foreach"}),          array_foreach);
-    DECLARE_VM_BUILTIN(name({"array", "iterate"}),          array_iterate);
-    DECLARE_VM_CASES_BUILTIN(name({"array", "cases_on"}),   array_cases_on);
+    DECLARE_VM_BUILTIN(name({"d_array", "foreach"}),        d_array_foreach);
+    DECLARE_VM_BUILTIN(name({"d_array", "iterate"}),        d_array_iterate);
+    DECLARE_VM_CASES_BUILTIN(name({"d_array", "cases_on"}), d_array_cases_on);
 }
 
 void finalize_vm_array() {
 }
 
 void initialize_vm_array_builtin_idxs() {
-    g_array_read_idx = *get_vm_builtin_idx(name({"array", "read"}));
+    g_array_read_idx = *get_vm_builtin_idx(name({"d_array", "read"}));
 }
 }
