library/init/data/array/basic.lean
@@ -4,127 +4,235 @@ Released under Apache 2.0 license as described in the file LICENSE.
 Authors: Leonardo de Moura, Mario Carneiro
 -/
 prelude
-import init.data.nat
-universes u w
+import init.data.nat init.data.bool init.ite_simp
+universes u v w
 
-structure array (α : Type u) (n : nat) :=
-(data : fin n → α)
+/- In the VM, d_array is implemented a persistent array. -/
+structure d_array (n : nat) (α : fin n → Type u) :=
+(data : Π i : fin n, α i)
 
-def mk_array {α} (n) (v : α) : array α n :=
-{data := λ _, v}
+namespace d_array
+variables {n : nat} {α : fin n → Type u} {β : Type v}
 
-namespace array
-variables {α : Type u} {β : Type w} {n : nat}
-
-def nil {α} : array α 0 :=
+def nil {α} : d_array 0 α :=
 {data := λ ⟨x, h⟩, absurd h (nat.not_lt_zero x)}
 
-def read (a : array α n) (i : fin n) : α :=
+/- has builtin VM implementation -/
+def read (a : d_array n α) (i : fin n) : α i :=
 a.data i
 
-def read' [inhabited α] (a : array α n) (i : nat) : α :=
-if h : i < n then a.read ⟨i,h⟩ else default α
+/- has builtin VM implementation -/
+def write (a : d_array n α) (i : fin n) (v : α i) : d_array n α :=
+{data := λ j, if h : i = j then eq.rec_on h v else a.read j}
 
-def write (a : array α n) (i : fin n) (v : α) : array α n :=
-{data := λ j, if i = j then v else a.read j}
-
-def write' (a : array α n) (i : nat) (v : α) : array α n :=
-if h : i < n then a.write ⟨i, h⟩ v else a
-
-lemma read_eq_read' [inhabited α] (a : array α n) (i : nat) (h : i < n) : read a ⟨i, h⟩ = read' a i :=
-by unfold read'; rw [dif_pos h]
-
-lemma write_eq_write' (a : array α n) (i : nat) (h : i < n) (v : α) : write a ⟨i, h⟩ v = write' a i v :=
-by unfold write'; rw [dif_pos h]
-
-lemma push_back_idx {j n} (h₁ : j < n + 1) (h₂ : j ≠ n) : j < n :=
-nat.lt_of_le_and_ne (nat.le_of_lt_succ h₁) h₂
-
-def push_back (a : array α n) (v : α) : array α (n+1) :=
-{data := λ ⟨j, h₁⟩, if h₂ : j = n then v else a.read ⟨j, push_back_idx h₁ h₂⟩}
-
-lemma pop_back_idx {j n} (h : j < n) : j < n + 1 :=
-nat.lt.step h
-
-def pop_back (a : array α (n+1)) : array α n :=
-{data := λ ⟨j, h⟩, a.read ⟨j, pop_back_idx h⟩}
-
-lemma lt_aux_1 {a b c : nat} (h : a + c < b) : a < b :=
-lt_of_le_of_lt (nat.le_add_right a c) h
-
-lemma lt_aux_2 {n} (h : n > 0) : n - 1 < n :=
-have h₁ : 1 > 0, from dec_trivial,
-nat.sub_lt h h₁
-
-lemma lt_aux_3 {n i} (h : i + 1 < n) : n - 2 - i < n  :=
-have n > 0,     from lt.trans (nat.zero_lt_succ i) h,
-have n - 2 < n, from nat.sub_lt this (dec_trivial),
-lt_of_le_of_lt (nat.sub_le _ _) this
-
-@[elab_as_eliminator]
-theorem write_ind (a : array α n) (i : fin n) (v : α) (C : fin n → α → Sort w)
-  (Hi : C i v) (Hj : ∀j, i ≠ j → C j (a.read j)) (j) : C j ((a.write i v).read j) :=
-show C j (if i = j then v else read a j), from
-if h : i = j then by rwa [if_pos h, ← h]
-else by rw [if_neg h]; exact Hj j h
-
-def iterate_aux (a : array α n) (f : fin n → α → β → β) : Π (i : nat), i ≤ n → β → β
+def iterate_aux (a : d_array n α) (f : Π i : fin n, α i → β → β) : Π (i : nat), i ≤ n → β → β
 | 0     h b := b
 | (j+1) h b :=
   let i : fin n := ⟨j, h⟩ in
   f i (a.read i) (iterate_aux j (le_of_lt h) b)
 
-def iterate (a : array α n) (b : β) (fn : fin n → α → β → β) : β :=
-iterate_aux a fn n (le_refl _) b
+/- has builtin VM implementation -/
+def iterate (a : d_array n α) (b : β) (f : Π i : fin n, α i → β → β) : β :=
+iterate_aux a f n (le_refl _) b
 
-def foreach (a : array α n) (f : fin n → α → α) : array α n :=
-iterate a a (λ i v a', a'.write i (f i v))
+/- has builtin VM implementation -/
+def foreach (a : d_array n α) (f : Π i : fin n, α i → α i) : d_array n α :=
+iterate a a $ λ i v a', a'.write i (f i v)
 
-def map (f : α → α) (a : array α n) : array α n :=
-foreach a (λ _, f)
+def map (f : Π i : fin n, α i → α i) (a : d_array n α) : d_array n α :=
+foreach a f
 
-def map₂ (f : α → α → α) (a b : array α n) : array α n :=
-foreach b (λ i, f (a.read i))
+def map₂ (f : Π i : fin n, α i → α i → α i) (a b : d_array n α) : d_array n α :=
+foreach b (λ i, f i (a.read i))
 
-def foldl (a : array α n) (b : β) (f : α → β → β) : β :=
-iterate a b (λ _, f)
+def foldl (a : d_array n α) (b : β) (f : Π i : fin n, α i → β → β) : β :=
+iterate a b f
 
-def rev_list (a : array α n) : list α :=
-a.foldl [] (λ v l, v :: l)
-
-def foldl_eq_aux (a : array α n) (b : β) (f : α → β → β) :
-  Π (i : nat) (h : i ≤ n), iterate_aux a (λ _, f) i h b = (iterate_aux a (λ _ v l, v :: l) i h []).foldr f b
-| 0     h := rfl
-| (j+1) h := congr_arg (f (read a ⟨j, h⟩)) (foldl_eq_aux j _)
-
-def foldl_eq (a : array α n) (b : β) (f : α → β → β) : a.foldl b f = a.rev_list.foldr f b :=
-foldl_eq_aux a b f _ _
-
-def rev_iterate_aux (a : array α n) (f : fin n → α → β → β) : Π (i : nat), i ≤ n → β → β
+def rev_iterate_aux (a : d_array n α) (f : Π i : fin n, α i → β → β) : Π (i : nat), i ≤ n → β → β
 | 0     h b := b
 | (j+1) h b :=
   let i : fin n := ⟨j, h⟩ in
   rev_iterate_aux j (le_of_lt h) (f i (a.read i) b)
 
-def rev_iterate (a : array α n) (b : β) (fn : fin n → α → β → β) : β :=
-rev_iterate_aux a fn n (le_refl _) b
+def rev_iterate (a : d_array n α) (b : β) (f : Π i : fin n, α i → β → β) : β :=
+rev_iterate_aux a f n (le_refl _) b
 
-def to_list (a : array α n) : list α :=
-a.rev_iterate [] (λ _ v l, v :: l)
+@[simp] lemma read_write (a : d_array n α) (i : fin n) (v : α i) : read (write a i v) i = v :=
+by simp [read, write]
 
-protected def mem (v : α) (a : array α n) : Prop := ∃i, read a i = v
+@[simp] lemma read_write_of_ne (a : d_array n α) {i j : fin n} (v : α i) : i ≠ j → read (write a i v) j = read a j :=
+by intro h; simp [read, write, h]
 
-instance : has_mem α (array α n) := ⟨array.mem⟩
+protected lemma ext {a b : d_array n α} (h : ∀ i, read a i = read b i) : a = b :=
+by cases a; cases b; congr; exact funext h
 
-theorem read_mem (a : array α n) (i) : read a i ∈ a := exists.intro i rfl
+protected lemma ext' {a b : d_array n α} (h : ∀ (i : nat) (h : i < n), read a ⟨i, h⟩ = read b ⟨i, h⟩) : a = b :=
+begin cases a, cases b, congr, apply funext, intro i, cases i, apply h end
 
-instance [has_repr α] : has_repr (array α n) :=
+protected def beq_aux [∀ i, decidable_eq (α i)] (a b : d_array n α) : Π (i : nat), i ≤ n → bool
+| 0     h := tt
+| (i+1) h := if a.read ⟨i, h⟩ = b.read ⟨i, h⟩ then beq_aux i (le_of_lt h) else ff
+
+protected def beq [∀ i, decidable_eq (α i)] (a b : d_array n α) : bool :=
+d_array.beq_aux a b n (le_refl _)
+
+lemma of_beq_aux_eq_tt [∀ i, decidable_eq (α i)] {a b : d_array n α} : ∀ (i : nat) (h : i ≤ n), d_array.beq_aux a b i h = tt →
+                       ∀ (j : nat) (h' : j < i), a.read ⟨j, lt_of_lt_of_le h' h⟩ = b.read ⟨j, lt_of_lt_of_le h' h⟩
+| 0     h₁ h₂ j h₃ := absurd h₃ (nat.not_lt_zero _)
+| (i+1) h₁ h₂ j h₃ :=
+  begin
+    have h₂' : read a ⟨i, h₁⟩ = read b ⟨i, h₁⟩ ∧ d_array.beq_aux a b i _ = tt, {simp [d_array.beq_aux] at h₂, assumption},
+    have h₁' : i ≤ n, from le_of_lt h₁,
+    have ih  : ∀ (j : nat) (h' : j < i), a.read ⟨j, lt_of_lt_of_le h' h₁'⟩ = b.read ⟨j, lt_of_lt_of_le h' h₁'⟩, from of_beq_aux_eq_tt i h₁' h₂'.2,
+    by_cases j = i with hji,
+    { subst hji, exact h₂'.1 },
+    { have j_lt_i : j < i, from lt_of_le_of_ne (nat.le_of_lt_succ h₃) hji,
+      exact ih j j_lt_i }
+  end
+
+lemma of_beq_eq_tt [∀ i, decidable_eq (α i)] {a b : d_array n α} : d_array.beq a b = tt → a = b :=
+begin
+  unfold d_array.beq,
+  intro h,
+  have : ∀ (j : nat) (h : j < n), a.read ⟨j, h⟩ = b.read ⟨j, h⟩, from
+    of_beq_aux_eq_tt n (le_refl _) h,
+  apply d_array.ext' this
+end
+
+lemma of_beq_aux_eq_ff [∀ i, decidable_eq (α i)] {a b : d_array n α} : ∀ (i : nat) (h : i ≤ n), d_array.beq_aux a b i h = ff →
+                       ∃ (j : nat) (h' : j < i), a.read ⟨j, lt_of_lt_of_le h' h⟩ ≠ b.read ⟨j, lt_of_lt_of_le h' h⟩
+| 0     h₁ h₂ := begin simp [d_array.beq_aux] at h₂, contradiction end
+| (i+1) h₁ h₂ :=
+  begin
+    have h₂' : read a ⟨i, h₁⟩ ≠ read b ⟨i, h₁⟩ ∨ d_array.beq_aux a b i _ = ff, {simp [d_array.beq_aux] at h₂, assumption},
+    cases h₂' with h h,
+    { existsi i, existsi (nat.lt_succ_self _), exact h },
+    { have h₁' : i ≤ n, from le_of_lt h₁,
+      have ih : ∃ (j : nat) (h' : j < i), a.read ⟨j, lt_of_lt_of_le h' h₁'⟩ ≠ b.read ⟨j, lt_of_lt_of_le h' h₁'⟩, from of_beq_aux_eq_ff i h₁' h,
+      cases ih with j ih,
+      cases ih with h' ih,
+      existsi j, existsi (nat.lt_succ_of_lt h'),
+      exact ih }
+  end
+
+lemma of_beq_eq_ff [∀ i, decidable_eq (α i)] {a b : d_array n α} : d_array.beq a b = ff → a ≠ b :=
+begin
+  unfold d_array.beq,
+  intros h hne,
+  have : ∃ (j : nat) (h' : j < n), a.read ⟨j, h'⟩ ≠ b.read ⟨j, h'⟩, from of_beq_aux_eq_ff n (le_refl _) h,
+  cases this with j this,
+  cases this with h' this,
+  subst hne,
+  contradiction
+end
+
+instance [∀ i, decidable_eq (α i)] : decidable_eq (d_array n α) :=
+λ a b, if h : d_array.beq a b = tt then is_true (of_beq_eq_tt h) else is_false (of_beq_eq_ff (eq_ff_of_not_eq_tt h))
+
+end d_array
+
+def array (n : nat) (α : Type u) : Type u :=
+d_array n (λ _, α)
+
+/- has builtin VM implementation -/
+def mk_array {α} (n) (v : α) : array n α :=
+{data := λ _, v}
+
+namespace array
+variables {n : nat} {α : Type u} {β : Type v}
+
+def nil {α} : array 0 α :=
+d_array.nil
+
+def read (a : array n α) (i : fin n) : α :=
+d_array.read a i
+
+def write (a : array n α) (i : fin n) (v : α) : array n α :=
+d_array.write a i v
+
+def iterate (a : array n α) (b : β) (f : fin n → α → β → β) : β :=
+d_array.iterate a b f
+
+def foreach (a : array n α) (f : fin n → α → α) : array n α :=
+iterate a a (λ i v a', a'.write i (f i v))
+
+def map (f : α → α) (a : array n α) : array n α :=
+foreach a (λ _, f)
+
+def map₂ (f : α → α → α) (a b : array n α) : array n α :=
+foreach b (λ i, f (a.read i))
+
+def foldl (a : array n α) (b : β) (f : α → β → β) : β :=
+iterate a b (λ _, f)
+
+def rev_list (a : array n α) : list α :=
+a.foldl [] (::)
+
+def rev_iterate (a : array n α) (b : β) (f : fin n → α → β → β) : β :=
+d_array.rev_iterate a b f
+
+def rev_foldl (a : array n α) (b : β) (f : α → β → β) : β :=
+rev_iterate a b (λ _, f)
+
+def to_list (a : array n α) : list α :=
+a.rev_foldl [] (::)
+
+lemma push_back_idx {j n} (h₁ : j < n + 1) (h₂ : j ≠ n) : j < n :=
+nat.lt_of_le_and_ne (nat.le_of_lt_succ h₁) h₂
+
+/- has builtin VM implementation -/
+def push_back (a : array n α) (v : α) : array (n+1) α :=
+{data := λ ⟨j, h₁⟩, if h₂ : j = n then v else a.read ⟨j, push_back_idx h₁ h₂⟩}
+
+lemma pop_back_idx {j n} (h : j < n) : j < n + 1 :=
+nat.lt.step h
+
+/- has builtin VM implementation -/
+def pop_back (a : array (n+1) α) : array n α :=
+{data := λ ⟨j, h⟩, a.read ⟨j, pop_back_idx h⟩}
+
+protected def mem (v : α) (a : array n α) : Prop :=
+∃ i : fin n, read a i = v
+
+instance : has_mem α (array n α) := ⟨array.mem⟩
+
+theorem read_mem (a : array n α) (i) : read a i ∈ a :=
+exists.intro i rfl
+
+instance [has_repr α] : has_repr (array n α) :=
 ⟨repr ∘ to_list⟩
 
-meta instance [has_to_format α] : has_to_format (array α n) :=
+meta instance [has_to_format α] : has_to_format (array n α) :=
 ⟨to_fmt ∘ to_list⟩
 
-meta instance [has_to_tactic_format α] : has_to_tactic_format (array α n) :=
+meta instance [has_to_tactic_format α] : has_to_tactic_format (array n α) :=
 ⟨tactic.pp ∘ to_list⟩
+
+@[simp] lemma read_write (a : array n α) (i : fin n) (v : α) : read (write a i v) i = v :=
+d_array.read_write a i v
+
+@[simp] lemma read_write_of_ne (a : array n α) {i j : fin n} (v : α) : i ≠ j → read (write a i v) j = read a j :=
+d_array.read_write_of_ne a v
+
+def read' [inhabited β] (a : array n β) (i : nat) : β :=
+if h : i < n then a.read ⟨i,h⟩ else default β
+
+def write' (a : array n α) (i : nat) (v : α) : array n α :=
+if h : i < n then a.write ⟨i, h⟩ v else a
+
+lemma read_eq_read' [inhabited α] (a : array n α) {i : nat} (h : i < n) : read a ⟨i, h⟩ = read' a i :=
+by simp [read', h]
+
+lemma write_eq_write' (a : array n α) {i : nat} (h : i < n) (v : α) : write a ⟨i, h⟩ v = write' a i v :=
+by simp [write', h]
+
+protected lemma ext {a b : array n α} (h : ∀ i, read a i = read b i) : a = b :=
+d_array.ext h
+
+protected lemma ext' {a b : array n α} (h : ∀ (i : nat) (h : i < n), read a ⟨i, h⟩ = read b ⟨i, h⟩) : a = b :=
+d_array.ext' h
+
+instance [decidable_eq α] : decidable_eq (array n α) :=
+begin unfold array, apply_instance end
 
 end array
