library/data/buffer.lean
@@ -5,12 +5,12 @@ Authors: Leonardo de Moura
 -/
 universes u w
 
-def buffer (α : Type u) := Σ n, array α n
+def buffer (α : Type u) := Σ n, array n α
 
 def mk_buffer {α : Type u} : buffer α :=
 ⟨0, {data := λ i, fin.elim0 i}⟩
 
-def array.to_buffer {α : Type u} {n : nat} (a : array α n) : buffer α :=
+def array.to_buffer {α : Type u} {n : nat} (a : array n α) : buffer α :=
 ⟨n, a⟩
 
 namespace buffer
@@ -22,7 +22,7 @@ mk_buffer
 def size (b : buffer α) : nat :=
 b.1
 
-def to_array (b : buffer α) : array α (b.size) :=
+def to_array (b : buffer α) : array (b.size) α :=
 b.2
 
 def push_back : buffer α → α → buffer α
@@ -63,13 +63,25 @@ def append_list {α : Type u} : buffer α → list α → buffer α
 def append_string (b : buffer char) (s : string) : buffer char :=
 b.append_list s.to_list
 
-def append_array {α : Type u} {n : nat} (nz : n > 0) : buffer α → array α n → ∀ i : nat, i < n → buffer α
+lemma lt_aux_1 {a b c : nat} (h : a + c < b) : a < b :=
+lt_of_le_of_lt (nat.le_add_right a c) h
+
+lemma lt_aux_2 {n} (h : n > 0) : n - 1 < n :=
+have h₁ : 1 > 0, from dec_trivial,
+nat.sub_lt h h₁
+
+lemma lt_aux_3 {n i} (h : i + 1 < n) : n - 2 - i < n  :=
+have n > 0,     from lt.trans (nat.zero_lt_succ i) h,
+have n - 2 < n, from nat.sub_lt this (dec_trivial),
+lt_of_le_of_lt (nat.sub_le _ _) this
+
+def append_array {α : Type u} {n : nat} (nz : n > 0) : buffer α → array n α → ∀ i : nat, i < n → buffer α
 | ⟨m, b⟩ a 0     _ :=
-  let i : fin n := ⟨n - 1, array.lt_aux_2 nz⟩ in
+  let i : fin n := ⟨n - 1, lt_aux_2 nz⟩ in
   ⟨m+1, b.push_back (a.read i)⟩
 | ⟨m, b⟩ a (j+1) h :=
-  let i : fin n := ⟨n - 2 - j, array.lt_aux_3 h⟩ in
-  append_array ⟨m+1, b.push_back (a.read i)⟩ a j (array.lt_aux_1 h)
+  let i : fin n := ⟨n - 2 - j, lt_aux_3 h⟩ in
+  append_array ⟨m+1, b.push_back (a.read i)⟩ a j (lt_aux_1 h)
 
 protected def append {α : Type u} : buffer α → buffer α → buffer α
 | b ⟨0, a⟩   := b
