library/init/data/array/slice.lean
@@ -10,26 +10,26 @@ variables {α : Type u} {n : nat}
 
 namespace array
 
-def slice (a : array α n) (k l : nat) (h₁ : k ≤ l) (h₂ : l ≤ n) : array α (l - k) :=
+def slice (a : array n α) (k l : nat) (h₁ : k ≤ l) (h₂ : l ≤ n) : array (l - k) α :=
 ⟨ λ ⟨ i, hi ⟩, a.read ⟨ i + k,
   calc i + k < (l - k) + k : add_lt_add_right hi _
          ... = l : nat.sub_add_cancel h₁
          ... ≤ n : h₂⟩ ⟩
 
-def take (a : array α n) (m : nat) (h : m ≤ n) : array α m :=
+def take (a : array n α) (m : nat) (h : m ≤ n) : array m α :=
 cast (by simp) $ a.slice 0 m (nat.zero_le _) h
 
-def drop (a : array α n) (m : nat) (h : m ≤ n) : array α (n-m) :=
+def drop (a : array n α) (m : nat) (h : m ≤ n) : array (n-m) α :=
 a.slice m n h (le_refl _)
 
 private lemma sub_sub_cancel (m n : ℕ) (h : m ≤ n) : n - (n - m) = m :=
 calc n - (n - m) = (n - m) + m - (n - m) : by rw nat.sub_add_cancel; assumption
              ... = m : nat.add_sub_cancel_left _ _
 
-def take_right (a : array α n) (m : nat) (h : m ≤ n) : array α m :=
+def take_right (a : array n α) (m : nat) (h : m ≤ n) : array m α :=
 cast (by simp [*, sub_sub_cancel]) $ a.drop (n - m) (nat.sub_le _ _)
 
-def reverse (a : array α n) : array α n :=
+def reverse (a : array n α) : array n α :=
 ⟨ λ ⟨ i, hi ⟩, a.read ⟨ n - (i + 1),
   begin apply nat.sub_lt_of_pos_le, apply nat.zero_lt_succ, assumption end ⟩ ⟩
 
