tests/lean/run/array1.lean
@@ -1,24 +1,24 @@
-#check @array.mk
+#check @d_array.mk
 
 #eval mk_array 4 1
 
-def v : array nat 10 :=
-@array.mk nat 10 (λ ⟨i, _⟩, i)
+def v : array 10 nat :=
+@d_array.mk 10 (λ _, nat) (λ ⟨i, _⟩, i)
 
 #eval array.map (+10) v
 
-def w : array nat 10 :=
+def w : array 10 nat :=
 (mk_array 9 1)^.push_back 3
 
 def f : fin 10 → nat :=
-array.cases_on w (λ f, f)
+d_array.cases_on w (λ f, f)
 
 #eval f ⟨9, dec_trivial⟩
 #eval f ⟨2, dec_trivial⟩
 
 #eval (((mk_array 1 1)^.push_back 2)^.push_back 3)^.foldl 0 (+)
 
-def array_sum {n} (a : array nat n) : nat :=
+def array_sum {n} (a : array n nat) : nat :=
 a^.foldl 0 (+)
 
 #eval array_sum (mk_array 10 1)
