tests/lean/run/eq_cases_on.lean
@@ -1,5 +1,5 @@
-def g {n m : nat} (v : array nat (n + m)) : array nat (m + n) :=
+def g {n m : nat} (v : array (n + m) nat) : array (m + n) nat :=
 eq.rec_on (add_comm n m) v -- Worked before
 
-def f {n m : nat} (v : array nat (n + m)) : array nat (m + n) :=
+def f {n m : nat} (v : array (n + m) nat) : array (m + n) nat :=
 eq.cases_on (add_comm n m) v -- eq.cases_on was not being erased
