tests/lean/task.lean
@@ -1,7 +1,7 @@
 run_cmd tactic.run_async (tactic.trace
   "trace message from a different task")
 
-def {u} foo {α : Type u} {n : ℕ} : array α (0+n) → array α n :=
+def {u} foo {α : Type u} {n : ℕ} : array (0+n) α → array n α :=
 if n = 0 then
   λ v, cast (by async { simp }) v
 else
